examples/sum.v
@@ -1,0 +1,158 @@
+From Coq Require Import
+     Morphisms
+     Program.
+
+(* TODO: Move this in the library  *)
+
+(** * The Category of Functions *)
+
+(* id : A -> A
+   compose : (B -> C) -> (A -> B) -> (A -> C)
+   Infix "∘" = compose
+
+   compose_id_right : f ∘ id = f
+   compose_id_left : id ∘ f = f
+   compose_assoc : (f ∘ g) ∘ h = f ∘ (g ∘ h)
+ *)
+
+Hint Rewrite @compose_id_left : cat.
+Hint Rewrite @compose_id_right : cat.
+
+(** Extensional function equality *)
+Definition eqeq {A B} := (@eq A ==> @eq B)%signature.
+
+Instance Equivalence_eqeq {A B} : Equivalence (@eqeq A B).
+Proof.
+  constructor; cbv; intros; subst; auto.
+  - symmetry; auto.
+  - etransitivity; auto.
+Qed.
+
+Instance eq_compose {A B C} :
+  Proper (eqeq ==> eqeq ==> eqeq) (@compose A B C).
+Proof. cbv; auto. Qed.
+
+(** * Diagramatic/categorical sum combinators. *)
+
+Definition sum_elim {A B C} (f : A -> C) (g : B -> C) : A + B -> C :=
+  fun x =>
+    match x with
+    | inl a => f a
+    | inr b => g b
+    end.
+
+Definition sum_bimap {A B C D} (f : A -> B) (g : C -> D) :
+  A + C -> B + D :=
+  sum_elim (inl ∘ f) (inr ∘ g).
+
+Definition sum_map_l {A B C} (f : A -> B) : A + C -> B + C :=
+  sum_bimap f id.
+
+Definition sum_map_r {A B C} (f : A -> B) : C + A -> C + B :=
+  sum_bimap id f.
+
+Definition sum_assoc_r {A B C} (abc : (A + B) + C) : A + (B + C) :=
+  match abc with
+  | inl (inl a) => inl a
+  | inl (inr b) => inr (inl b)
+  | inr c => inr (inr c)
+  end.
+
+Definition sum_comm {A B} : A + B -> B + A :=
+  sum_elim inr inl.
+
+Definition sum_assoc_l {A B C} (abc : A + (B + C)) : (A + B) + C :=
+  match abc with
+  | inl a => inl (inl a)
+  | inr (inl b) => inl (inr b)
+  | inr (inr c) => inr c
+  end.
+
+Definition sum_merge {A} : A + A -> A := sum_elim id id.
+
+(** ** Equational theory *)
+
+Lemma compose_sum_elim {A B C D} (ac : A -> C) (bc : B -> C) (cd : C -> D) :
+  eqeq (cd ∘ sum_elim ac bc)
+       (sum_elim (cd ∘ ac) (cd ∘ bc)).
+Proof.
+  intros [] ? []; auto.
+Qed.
+
+Lemma sum_elim_inl {A B C} (f : A -> C) (g : B -> C) :
+  sum_elim f g ∘ inl = f.
+Proof. reflexivity. Qed.
+
+Lemma sum_elim_inr {A B C} (f : A -> C) (g : B -> C) :
+  sum_elim f g ∘ inr = g.
+Proof. reflexivity. Qed.
+
+Lemma sum_elim_inl' {A B C D} (f : A -> C) (g : B -> C) (h : D -> A) :
+  sum_elim f g ∘ (inl ∘ h) = f ∘ h.
+Proof. reflexivity. Qed.
+
+Lemma sum_elim_inr' {A B C D} (f : A -> C) (g : B -> C) (h : D -> B) :
+  sum_elim f g ∘ (inr ∘ h) = g ∘ h.
+Proof. reflexivity. Qed.
+
+Lemma unfold_sum_assoc_r {A B C} :
+  @sum_assoc_r A B C = sum_elim (sum_elim inl (inr ∘ inl)) (inr ∘ inr).
+Proof. cbv; auto. Qed.
+
+Instance eqeq_sum_elim {A B C} :
+  Proper (eqeq ==> eqeq ==> eqeq) (@sum_elim A B C).
+Proof. cbv; intros; subst; destruct _; auto. Qed.
+
+Hint Rewrite @sum_elim_inl : sum_elim.
+Hint Rewrite @sum_elim_inr : sum_elim.
+Hint Rewrite @sum_elim_inl' : sum_elim.
+Hint Rewrite @sum_elim_inr' : sum_elim.
+
+(** ** Automatic solver of reassociating sums *)
+
+Class ReSum (A B : Type) :=
+  resum : A -> B.
+
+Instance ReSum_id A : ReSum A A := id.
+Instance ReSum_sum A B C `{ReSum A C} `{ReSum B C} : ReSum (A + B) C :=
+  sum_elim resum resum.
+Instance ReSum_inl A B C `{ReSum A B} : ReSum A (B + C) :=
+  inl ∘ resum.
+Instance ReSum_inr A B C `{ReSum A B} : ReSum A (C + B) :=
+  inr ∘ resum.
+
+(* Usage template:
+
+[[
+Opaque compose.
+Opaque id.
+Opaque sum_elim.
+
+Definition f {X Y Z} : complex_sum -> another_complex_sum :=
+  Eval compute in resum.
+
+Transparent compose.
+Transparent id.
+Transparent sum_elim.
+]]
+*)
+
+(** * Bijections *)
+
+Class Iso {A B} (f : A -> B) (f' : B -> A) : Type :=
+  { iso_ff' : forall a, f' (f a) = a;
+    iso_f'f : forall b, f (f' b) = b;
+  }.
+
+Instance Iso_sum_assoc_l {A B C} : Iso (@sum_assoc_l A B C) sum_assoc_r := {}.
+Proof.
+  - destruct 0 as [| []]; auto.
+  - destruct 0 as [[] |]; auto.
+Qed.
+
+Instance Iso_sum_assoc_r {A B C} : Iso (@sum_assoc_r A B C) sum_assoc_l := {}.
+Proof.
+  - destruct 0 as [[] |]; auto.
+  - destruct 0 as [| []]; auto.
+Qed.
+
